.travis-ci.sh
@@ -1,15 +1,10 @@
+#!/usr/bin/env bash
+
 set -ev
 
-opam init --yes --no-setup
 eval $(opam config env)
 
-opam repo add coq-released https://coq.inria.fr/opam/released
-opam repo add coq-core-dev https://coq.inria.fr/opam/core-dev
-opam repo add coq-extra-dev https://coq.inria.fr/opam/extra-dev
+opam update
 
-opam pin add coq $COQ_VERSION --kind=version --yes
-opam pin add coq-mathcomp-ssreflect $SSREFLECT_VERSION --kind=version --yes --verbose
-
-opam pin add Heaps --yes --verbose
-opam pin add Core --yes --verbose
+opam pin add Core disel --yes --verbose
 make -j4 -C Examples
